---
title: "The Ext and Tor derived functors: Ext computations (2/?)"
date: 2026-02-01 12:20:00 +0100
categories: [Homological Algebra?]
tags: [Abstract Nonsense, Categorical Bullsh*t]
math: true
---

$$
\newcommand{\t}[1]{\text{#1}}
\newcommand{\Ext}{\text{Ext}}
\newcommand{\Tor}{\text{Tor}}
\newcommand{\Hom}{\text{Hom}}
\newcommand{\ker}{\text{ker}}
\newcommand{\Syz}{\text{Syz}}
\newcommand{\im}{\text{im}}
$$

In the last post, I talked about the "general" definition of $\Ext$ (in particular over $\t{R-Mod}$). Seeing as it was largely purely theoretical, I would like to go over some computations for $\Ext^1$ in particular.

Perhaps one of the most typical examples of the usage of this functor is the free/syzygytic resolution of an R-module. Suppose $M$ is a module over the polynomial ring $k\[x_1, \ldots x_n \]$. By Hilbert's syzygy theorem, if $M$ is finitely generated over a polynomial ring in $n$ indeterminates over a field $k$, then the $n^{th}$ syzygy module $\text{Syz}^n (M)$ is a free module (recall that in $\text{R-Mod}$ free modules are projective!).
Of course, to make any sense of this, it is necessary that a syzygy module is even defined. 

For the sake of sanity, we work over the ring $R = \mathbb{C}\[x_1, \ldots x_n\]$, and $M$ be a finitely generated $R$-module. Suppose the set $\{a_1, a_2, \ldots, a_k\} \subset M$ generates $M$. Then we may construct a sequence of $R$-linear maps (module homomorphisms) 

![Syzygytic is a funny word](/assets/img/syzygytic.png)

where $\varphi$ sends the basis element $e_i$ of $R^k$ to the generators $a_i$ of $M$. Rather anticlimactically, $\t{Syz}^1(M) := \ker(\varphi)$, read as the first syzygy module of $M$. An element of $R^k$ can be expressed as a linear combination of its basis elements, so we may write $r = \lambda_1e_1 + \lambda_2 e_2 + \ldots + \lambda_k e_k \in R^k$. Then, since $\varphi$ is $R$-linear (a homomorphism), 
$\varphi(r) = \varphi(\lambda_1e_1 + \lambda_2 e_2 + \ldots + \lambda_k e_k) = \lambda_1 \varphi(e_1) + \ldots + \lambda_k \varphi(e_k) = \lambda_1 a_1 + \lambda_2 a_2 + \ldots \lambda_k a_k$. Now, $\Syz^1(M) = \ker(\varphi)$ reads as the equation $\lambda_1 a_1 + \lambda_2 a_2 + \ldots + \lambda_k a_k = 0$, which constitutes a relation between generators of $M$.
Since, by Hilbert's basis theorem, $\Syz^1(M)$ is finitely generated, we may again choose a set $\{m_1, m_2, \ldots m_l\}$ of generators. Then, we have another sequence of module homomorphisms:

![same thing but with a psi instead of a phi](/assets/img/2ndsyz.png)

Since $\psi$ sends the $j$-th basis vector of $R^l$ to the generator $m_j \in \ker(\varphi)$. Thus, 
$\im(\psi) = \ker(\varphi)$, and we can trivially map generators of $\ker(\varphi)$ to generators of $R^k$ (since $\ker(\varphi) \subseteq R^k$), we have the following exact sequence:

![Free resolution](/assets/img/freeres.png)

This sequence has length $n$ as per Hilbert's syzygy theorem.

To provide a concrete example, we consider $R = \mathbb{C}[x, y],$ and the module $M = R/(x,y)$. $M$ is generated by $1$.
We let our first element of the free resolution $F_0 = R$, with a map $\varphi: F_0 \to M$ via mapping $1 \mapsto \bar{1}$. The kernel of this map is simply the ideal $(x, y) \subset R$, so $\Syz^1(M) = \ker(\varphi) = (x,y)$. Then, we choose generators of $(x,y)$ being $m_1 = x, m_2 = y$. 
The next free module is $F_1 = R^2$, with a map $\psi: F_1 \to F_0$. Suppose $f_1, f_2$ are generators of $R^2$. Then, we have $f_1 \mapsto x, f_2 \mapsto y$ via $\psi$. To find $\ker(\psi)$, for a general element $(a,b) \in F_1 = R^2$ which corresponds to a linear combination $af_1 + bf_2$, $\psi(af_1 + bf_2) = ax + by \in R$. Evidently then, $\\{ \ker(\psi) =  (a,b) \mid ax + by = 0 \\}$, with solution $r(-y, x)$, for some $r \in R$, meaning that $\ker(\psi)$ is the submodule generated by the element $(-y, x)$. Lastly, we want a module $F_2$ that surjects onto $\ker(\psi)$. Since this kernel is generated by one element, we may take $F_2 = R$ with the basis element $g_1$ with a mapping $\theta$ such that  $g_1 \mapsto (-y, x)$. This map is injective because $(-y, x)$ genertes the kernel of $\psi$, so no nonzero element of $F_2$ maps to $0$, meaning that the kernel of this map is $0$. This corresponds to $\Syz^3(M) = \ker(\theta) = 0$, which is trivially free. Thus, our resolution terminates here.
Here is a diagram of the resolution:

![concrete free resolution](/assets/img/concreteres.png)

We proceed to computing $\Ext^1(M, A)$, where $M$ is the module specified above, and A can be any $R$-module. The simplest choice is setting $A = R$ itself. 
To compute $\Ext^1$, we must first apply the contravariant $\Hom(-, R)$, yielding the following sequence:

![homified](/assets/img/freehom.png)

Over $R$, $\Hom_R(R, R) \cong R$, and $\Hom_R(R^2, R) \cong R^2$, so we may rewrite this as:
![isoed](/assets/img/isoed.png)

Then, $$\Ext^1_R(M, A) = \ker(\theta^{*}) / \im(\psi^{*})$$. 

For a map $f: R \to R$, we define $\psi^*(f) = f \circ \psi$, which takes an element of $\Hom(R,R)$ and yields an element of $\Hom_R(R^2, R)$ (you may check this using the typings of the morphisms). 

Similarly, $\theta^* (g) = g \circ \theta$, which takes an element of $\Hom(R^2, R)$ and produces an element of $\Hom(R, R)$ (you may also check this). Concretely, $\theta^* (g)$ sends $x \in R$ to $g(\theta(x))$.
To find $\ker(\theta^*)$, we solve $$\theta^*(g_1, g_2) = -yg_1 + xg_2 = 0 \implies xg_2 = yg_1$$. 
Over $R$, a solution is $g_1 = xh$ and $g_2 = yh$ for some $h \in R$. Hence,
$$\ker(\theta^*) = \{(xh, yh) \mid h \in R\} \cong R \cdot (x,y)$$. For $$\im(\psi^*),$$ $$\psi^* (f) = (fx, fy) = f \cdot (x,y), f \in R$$, which is precisely the same as the kernel. 
Finally, we may write $$\Ext^1_R (M, R) = R \cdot (x,y) / R \cdot (x,y) = 0.$$
It makes sense that the $\Ext^1$ group is trivial here, since every short exact sequence of modules of the form

$$0 \to A \to E \to M \to 0$$

splits, meaning that $E \cong A \oplus M$, so there cannot be any nontrivial extensions of $M$. 

A second example to compute $\Ext^1$ uses $R = \mathbb{Z}, M = \mathbb{Z}/n\mathbb{Z}, A = \mathbb{Z}$.
The free resolution of $M$ is

$$0 \to \mathbb{Z} \overset{\cdot n}{\to} \mathbb{Z} \to \mathbb{Z}/n\mathbb{Z} \to 0.$$ 

Applying contravariant $\Hom_\mathbb{Z}(-, \mathbb{Z}),$

$$0 \gets\Hom_\mathbb{Z}(\mathbb{Z}, \mathbb{Z}) \overset{\cdot n}{\gets} \Hom_\mathbb{Z}(\mathbb{Z}, \mathbb{Z})$$

Over $\mathbb{Z}, \Hom_\mathbb{Z}(\mathbb{Z}, \mathbb{Z}) \cong \mathbb{Z}$, meaning the sequence above is equivalent to

$$0 \gets \mathbb{Z} \overset{\cdot n }{\gets} \mathbb{Z}$$


so $$\Ext^1_\mathbb{Z}(M, \mathbb{Z}) = \ker(0)/\im(\cdot n) = \mathbb{Z}/ n\mathbb{Z}.$$

I think that's probably enough examples for this post.